chore: fix (PersistentHashMap.insert k v).size
correctier

more thorough test

correction

src/Lean/Data/PersistentHashMap.lean
@@ -74,20 +74,24 @@ private theorem size_set {ks : Array α} {vs : Array β} (h : ks.size = vs.size)
 private theorem size_push {ks : Array α} {vs : Array β} (h : ks.size = vs.size) (k : α) (v : β) : (ks.push k).size = (vs.push v).size := by
   simp [h]
 
-partial def insertAtCollisionNodeAux [BEq α] : CollisionNode α β → Nat → α → β → CollisionNode α β
+instance : Inhabited (CollisionNode α β × Bool) where
+  default := (⟨Node.collision #[] #[] rfl, .mk _ _ _⟩, true)
+
+partial def insertAtCollisionNodeAux [BEq α] : CollisionNode α β → Nat → α → β → CollisionNode α β × Bool
   | n@⟨Node.collision keys vals heq, _⟩, i, k, v =>
     if h : i < keys.size then
       let idx : Fin keys.size := ⟨i, h⟩;
       let k' := keys.get idx;
       if k == k' then
          let j : Fin vals.size := ⟨i, by rw [←heq]; assumption⟩
-         ⟨Node.collision (keys.set idx k) (vals.set j v) (size_set heq idx j k v), IsCollisionNode.mk _ _ _⟩
+         (⟨Node.collision (keys.set idx k) (vals.set j v) (size_set heq idx j k v), IsCollisionNode.mk _ _ _⟩, true)
       else insertAtCollisionNodeAux n (i+1) k v
     else
-      ⟨Node.collision (keys.push k) (vals.push v) (size_push heq k v), IsCollisionNode.mk _ _ _⟩
+      (⟨Node.collision (keys.push k) (vals.push v) (size_push heq k v), IsCollisionNode.mk _ _ _⟩, false)
   | ⟨Node.entries _, h⟩, _, _, _ => nomatch h
 
-def insertAtCollisionNode [BEq α] : CollisionNode α β → α → β → CollisionNode α β :=
+/-- Inserts a key-value pair into a CollisionNode, also returning whether an existing value was replaced. -/
+def insertAtCollisionNode [BEq α] : CollisionNode α β → α → β → CollisionNode α β × Bool  :=
   fun n k v => insertAtCollisionNodeAux n 0 k v
 
 def getCollisionNodeSize : CollisionNode α β → Nat
@@ -101,10 +105,14 @@ def mkCollisionNode (k₁ : α) (v₁ : β) (k₂ : α) (v₂ : β) : Node α β
   let vs := (vs.push v₁).push v₂
   Node.collision ks vs rfl
 
-partial def insertAux [BEq α] [Hashable α] : Node α β → USize → USize → α → β → Node α β
+/--
+Inserts a key-value pair into a node, returning the new node,
+along with a `Bool` indicating whether an existing value was replaced.
+-/
+partial def insertAux [BEq α] [Hashable α] : Node α β → USize → USize → α → β → (Node α β × Bool)
   | Node.collision keys vals heq, _, depth, k, v =>
-    let newNode := insertAtCollisionNode ⟨Node.collision keys vals heq, IsCollisionNode.mk _ _ _⟩ k v
-    if depth >= maxDepth || getCollisionNodeSize newNode < maxCollisions then newNode.val
+    let (newNode, replaced) := insertAtCollisionNode ⟨Node.collision keys vals heq, IsCollisionNode.mk _ _ _⟩ k v
+    if depth >= maxDepth || getCollisionNodeSize newNode < maxCollisions then (newNode.val, replaced)
     else match newNode with
       | ⟨Node.entries _, h⟩ => nomatch h
       | ⟨Node.collision keys vals heq, _⟩ =>
@@ -115,22 +123,32 @@ partial def insertAux [BEq α] [Hashable α] : Node α β → USize → USize �
             let v := vals[i]
             let h := hash k |>.toUSize
             let h := div2Shift h (shift * (depth - 1))
-            traverse (i+1) (insertAux entries h depth k v)
+            -- We don't need to capture the `replaced` flag here,
+            -- as the result from `insertAtCollisionNode` already tells us if we are replacing a value.
+            let (entries', _) := insertAux entries h depth k v
+            traverse (i+1) entries'
           else
             entries
-        traverse 0 mkEmptyEntries
+        (traverse 0 mkEmptyEntries, replaced)
   | Node.entries entries, h, depth, k, v =>
     let j     := (mod2Shift h shift).toNat
-    Node.entries $ entries.modify j fun entry =>
-      match entry with
-      | Entry.null        => Entry.entry k v
-      | Entry.ref node    => Entry.ref $ insertAux node (div2Shift h shift) (depth+1) k v
+    -- We can't use `entries.modify` here, as we need to return `replaced`.
+    -- To ensure linearity, we use `swapAt!`.
+    let (entry, entries') := entries.swapAt! j .null
+    let (entry', replaced) := match entry with
+      | Entry.null        => (Entry.entry k v, false)
+      | Entry.ref node    =>
+        let r := insertAux node (div2Shift h shift) (depth+1) k v
+        (Entry.ref r.1, r.2)
       | Entry.entry k' v' =>
-        if k == k' then Entry.entry k v
-        else Entry.ref $ mkCollisionNode k' v' k v
+        if k == k' then (Entry.entry k v, true)
+        else (Entry.ref $ mkCollisionNode k' v' k v, false)
+    (Node.entries $ entries'.set! j entry', replaced)
 
 def insert {_ : BEq α} {_ : Hashable α} : PersistentHashMap α β → α → β → PersistentHashMap α β
-  | { root := n, size := sz }, k, v => { root := insertAux n (hash k |>.toUSize) 1 k v, size := sz + 1 }
+  | { root := n, size := sz }, k, v =>
+    let (node, replaced) := insertAux n (hash k |>.toUSize) 1 k v
+    { root := node, size := if replaced then sz else sz + 1 }
 
 partial def findAtAux [BEq α] (keys : Array α) (vals : Array β) (heq : keys.size = vals.size) (i : Nat) (k : α) : Option β :=
   if h : i < keys.size then
